{
 "cells": [
  {
   "cell_type": "markdown",
   "metadata": {},
   "source": [
    "# ANLY 561 HW\n",
    "\n",
    "Name:Yuqi Wang   \n",
    "NetID:yw545"
   ]
  },
  {
   "cell_type": "markdown",
   "metadata": {},
   "source": [
    "## Problem 1\n",
    "### Part (a)\n",
    "\n",
    "Observe that this program  \n",
    "$$\n",
    "\\max_{x\\in\\mathbb{R^2}}x_1 \\text{ subject to } x_2+(x_1-1)^3\\leq0, x_1\\geq0, x_2\\geq0.\n",
    "$$  \n",
    "is equivalent to the program  \n",
    "$$\n",
    "\\min_{x\\in\\mathbb{R^2}}-x_1 \\text{ subject to } x_2+(x_1-1)^3\\leq0, x_1\\geq0, x_2\\geq0.\n",
    "$$  \n",
    "Now we let $f(x_1,x_2)=-x_1$, $h_1(x_1,x_2)=x_2+(x_1-1)^3$, $h_2(x_1,x_2)=-x_1$, $h_3(x_1,x_2)=-x_2$, then we have  \n",
    "$$\n",
    "\\nabla f(x_1,x_2) = \\begin{pmatrix} -1 \\\\ 0 \\end{pmatrix}, \\nabla h_1(x_1,x_2) = \\begin{pmatrix} 3(x_1-1)^2 \\\\ 1 \\end{pmatrix}, \\nabla h_2(x_1,x_2) = \\begin{pmatrix} -1 \\\\ 0 \\end{pmatrix}, \\nabla h_3(x_1,x_2) = \\begin{pmatrix} 0 \\\\ -1 \\end{pmatrix}.\n",
    "$$  \n",
    "At $x=\\begin{pmatrix}1 \\\\ 0 \\end{pmatrix}$,  \n",
    "$$\n",
    "\\nabla h_1(1,0) = \\begin{pmatrix} 0 \\\\ 1 \\end{pmatrix}, \\nabla h_2(1,0) = \\begin{pmatrix} -1 \\\\ 0 \\end{pmatrix}, \\nabla h_3(1,0) = \\begin{pmatrix} 0 \\\\ -1 \\end{pmatrix}\n",
    "$$  \n",
    "So we can see that $\\nabla h_1(1,0)$ and $\\nabla h_3(1,0)$ are linearly dependent because if we form a eqution that $c_1 \\nabla h_1(1,0) + c_2 \\nabla h_3(1,0) = {\\bf 0}$, $c_1$ could be any number (so not necessary to be $0$), then $c_2=-c_1$ could satisfy the equation.  \n",
    "Since $\\nabla h_1(1,0)$ and $\\nabla h_3(1,0)$ are linearly dependent, the Linear Independence Constraint Qualification fails at $x=\\begin{pmatrix}1 \\\\ 0 \\end{pmatrix}$.  \n"
   ]
  },
  {
   "cell_type": "markdown",
   "metadata": {},
   "source": [
    "### Part (b) \n",
    "\n",
    "The KKT conditions:  \n",
    "(Stationarity)   \n",
    "$$\n",
    "-\\begin{pmatrix} -1 \\\\ 0 \\end{pmatrix} = \\lambda_1\\begin{pmatrix} 3(x_1-1)^2 \\\\ 1 \\end{pmatrix}+\\lambda_2\\begin{pmatrix} -1 \\\\ 0 \\end{pmatrix}+\\lambda_3\\begin{pmatrix} 0 \\\\ -1 \\end{pmatrix}\n",
    "$$  \n",
    "\n",
    "(Primal Feasibility)  \n",
    "$$\n",
    "h_1(x_1,x_2)=x_2+(x_1-1)^3\\leq 0,h_2(x_1,x_2)=-x_1\\leq 0,,h_3(x_1,x_2)=-x_2\\leq 0\n",
    "$$\n",
    "\n",
    "(Dual Feasibility)  \n",
    "$$\n",
    "\\lambda_1\\geq0, \\lambda_2\\geq0,\\lambda_3\\geq0\n",
    "$$\n",
    "\n",
    "(Complementary Slackness)\n",
    "$$\n",
    "\\lambda_1 h_1(x_1,x_2)= \\lambda_1 (x_2+(x_1-1)^3)=0, \\lambda_2 h_2(x_1,x_2) = \\lambda_2(-x_1)=0, \\lambda_3 h_3(x_1,x_2)= \\lambda_3(-x_2)=0\n",
    "$$"
   ]
  },
  {
   "cell_type": "markdown",
   "metadata": {},
   "source": [
    "### Part (c) \n",
    "\n",
    "As $x=\\begin{pmatrix}1 \\\\ 0 \\end{pmatrix}$,  \n",
    "$$\n",
    "-\\begin{pmatrix} -1 \\\\ 0 \\end{pmatrix} = \\lambda_1\\begin{pmatrix} 0 \\\\ 1 \\end{pmatrix}+\\lambda_2\\begin{pmatrix} -1 \\\\ 0 \\end{pmatrix}+\\lambda_3\\begin{pmatrix} 0 \\\\ -1 \\end{pmatrix}\n",
    "$$  \n",
    "implies that $\\lambda_2$ has to be $-1<0$, so it does not satisfy the Dual Feasibility. Therefore, $x=\\begin{pmatrix}1 \\\\ 0 \\end{pmatrix}$ does not satisfy the KKT conditions."
   ]
  },
  {
   "cell_type": "markdown",
   "metadata": {
    "collapsed": true
   },
   "source": [
    "### Part (d)\n",
    "\n",
    "Consider the program  \n",
    "$$\n",
    "\\max_{x\\in\\mathbb{R^2}}x_1 \\text{ subject to } x_2+(x_1-1)^3\\leq0, x_1\\geq0, x_2\\geq0.\n",
    "$$  \n",
    "and we suppose that $x=\\begin{pmatrix}1 \\\\ 0 \\end{pmatrix}$ is NOT the solution to the above program, then there must exist a $x^\\ast=\\begin{pmatrix}x_1^\\ast \\\\x_2^\\ast \\end{pmatrix}$ such that $x_2^\\ast+(x_1^\\ast-1)^3\\leq0$, $x_1^\\ast\\geq0$, $x_2^\\ast\\geq0$ and also $x_1^\\ast>1$. Since $x_1^\\ast>1$, then $(x_1^\\ast-1)^3>0$. If we want to satisfy $x_2^\\ast+(x_1^\\ast-1)^3\\leq0$, $x_2^\\ast$ has to be less than $0$. However, we also have a condition that $x_2^\\ast\\geq0$. Thus, we get a contradiction.  \n",
    "So $x=\\begin{pmatrix}1 \\\\ 0 \\end{pmatrix}$ is the solution to this program."
   ]
  },
  {
   "cell_type": "markdown",
   "metadata": {},
   "source": [
    "## Problem 2\n",
    "### Part (a)\n",
    "\n",
    "Consider the program  \n",
    "$$\n",
    "\\min_{x\\in\\mathbb{R^2}}3x_1^2-2x_1x_2+3x_2^2-2x_2x_3+3x_3^2 \\text{ subject to } 0\\leq x_1\\leq1, 0\\leq x_2\\leq1, 0\\leq x_3\\leq1\n",
    "$$  \n",
    "Now we let $f(x_1,x_2,x_3)=3x_1^2-2x_1x_2+3x_2^2-2x_2x_3+3x_3^2$, $h_1(x_1,x_2,x_3)=-x_1$, $h_2(x_1,x_2,x_3)=x_1-1$, $h_3(x_1,x_2,x_3)=-x_2$, $h_4(x_1,x_2,x_3)=x_2-1$, $h_5(x_1,x_2,x_3)=-x_3$, $h_6(x_1,x_2,x_3)=x_3-1$, then we have  \n",
    "$$\n",
    "\\nabla^2 f(x_1,x_2,x_3)=\\begin{pmatrix}\n",
    "6 & -2 & 0 \\\\\n",
    "-2 & 6 & -2 \\\\\n",
    "0 & -2 & 6\n",
    "\\end{pmatrix}\n",
    "$$  \n",
    "So $\\nabla^2 f$ has $1$ by $1$ leading principal minor: $6$.  \n",
    "$\\nabla^2 f$ has $2$ by $2$ leading principal minor: $6*6-(-2)(-2)=36-4=32$.  \n",
    "$\\nabla^2 f$ has $3$ by $3$ leading principal minor: $6*(6*6-(-2)(-2))-(-2)((-2)6-0)=192-24=168$.  \n",
    "By Sylvester's Criterion, $\\nabla^2 f(x_1,x_2,x_3)$ is positive definite. Then by Second Order Conditions for Convexity, $f(x_1,x_2,x_3)$ is strictly convex.  \n",
    "In addition, $h_1(x_1,x_2,x_3)=-x_1$, $h_2(x_1,x_2,x_3)=x_1-1$, $h_3(x_1,x_2,x_3)=-x_2$, $h_4(x_1,x_2,x_3)=x_2-1$, $h_5(x_1,x_2,x_3)=-x_3$, $h_6(x_1,x_2,x_3)=x_3-1$ are all affine so they are all convex. So the program is a convex program. And as $x=\\begin{pmatrix}0.5 \\\\ 0.5 \\\\ 0.5 \\end{pmatrix}$, it satisfies $h_1<0,h_2<0,h_3<0,h_4<0,h_5<0,h_6<0$ï¼Œwhich means that Slater's condition holds. Therefore, by the Sufficient Conditions for Convex Programming, the solution to this program must satisfy the KKT conditions.\n"
   ]
  },
  {
   "cell_type": "markdown",
   "metadata": {},
   "source": [
    "### Part (b) \n",
    "\n",
    "The KKT conditions:  \n",
    "(Stationarity)   \n",
    "$$\n",
    "-\\begin{pmatrix} 6x_1-2x_2 \\\\ -2x_1+6x_2-2x_3 \\\\ -2x_2+6x_3 \\end{pmatrix} = \\lambda_1\\begin{pmatrix} -1 \\\\ 0 \\\\ 0 \\end{pmatrix}+\\lambda_2\\begin{pmatrix} 1 \\\\ 0 \\\\ 0 \\end{pmatrix}+\\lambda_3\\begin{pmatrix} 0 \\\\ -1 \\\\ 0 \\end{pmatrix}+\\lambda_4\\begin{pmatrix} 0 \\\\ 1 \\\\ 0 \\end{pmatrix}+\\lambda_5\\begin{pmatrix} 0 \\\\ 0 \\\\ -1 \\end{pmatrix}+\\lambda_6\\begin{pmatrix} 0 \\\\ 0 \\\\ 1 \\end{pmatrix}\n",
    "$$  \n",
    "\n",
    "(Primal Feasibility)  \n",
    "$$\n",
    "h_1(x_1,x_2,x_3)=-x_1\\leq0, h_2(x_1,x_2,x_3)=x_1-1\\leq0, h_3(x_1,x_2,x_3)=-x_2\\leq0,\\\\\n",
    "h_4(x_1,x_2,x_3)=x_2-1\\leq0, h_5(x_1,x_2,x_3)=-x_3\\leq0, h_6(x_1,x_2,x_3)=x_3-1\\leq0\n",
    "$$\n",
    "\n",
    "(Dual Feasibility)  \n",
    "$$\n",
    "\\lambda_1\\geq0, \\lambda_2\\geq0,\\lambda_3\\geq0, \\lambda_4\\geq0, \\lambda_5\\geq0,\\lambda_6\\geq0\n",
    "$$\n",
    "\n",
    "(Complementary Slackness)\n",
    "$$\n",
    "\\lambda_1 h_1(x_1,x_2,x_3)= \\lambda_1 (-x_1)=0, \\lambda_2 h_2(x_1,x_2,x_3)= \\lambda_2(x_1-1)=0, \\lambda_3 h_3(x_1,x_2,x_3)= \\lambda_3(-x_2)=0, \\\\\n",
    "\\lambda_4 h_4(x_1,x_2,x_3) = \\lambda_4(x_2-1)=0,\\lambda_5 h_5(x_1,x_2,x_3)= \\lambda_5(-x_3)=0, \\lambda_6 h_6(x_1,x_2,x_3) = \\lambda_6(x_3-1)=0\n",
    "$$"
   ]
  },
  {
   "cell_type": "markdown",
   "metadata": {},
   "source": [
    "### Part (c) \n",
    "\n",
    "We have\n",
    "$$\n",
    "\\begin{pmatrix}\n",
    "2x_2-6x_1 = -\\lambda_1+\\lambda_2 & 2x_1-6x_2+2x_3 = -\\lambda_3+\\lambda_4 & 2x_2-6x_3 = -\\lambda_5+\\lambda_6 \\\\\n",
    "\\lambda_1(-x_1)=0 & \\lambda_2(x_1 -1)=0 & \\lambda_3(-x_2)=0 \\\\\n",
    "\\lambda_4(x_2 -1)=0 & \\lambda_5(-x_3)=0 & \\lambda_6(x_3 -1)=0\n",
    "\\end{pmatrix}\n",
    "$$  \n",
    "and  \n",
    "$$\n",
    "\\lambda_1\\geq0, \\lambda_2\\geq0,\\lambda_3\\geq0, \\lambda_4\\geq0, \\lambda_5\\geq0,\\lambda_6\\geq0 \\\\\n",
    "0\\leq x_1\\leq1, 0\\leq x_2\\leq1, 0\\leq x_3\\leq1\n",
    "$$  \n",
    "\n",
    "* Case 1:\n",
    "$x_1 = 0$, then $x_1-1 \\neq 0$, so $\\lambda_2=0$,  \n",
    "\n",
    " * Case 1-1:\n",
    " $x_2=0$, $x_3=0$, then $\\lambda_1=\\lambda_2=\\lambda_3=\\lambda_4=\\lambda_5=\\lambda_6=0$, it satisfies the KKT conditions.\n",
    "\n",
    " * Case 1-2:\n",
    " $x_2=0$, $x_3=1$, then $\\lambda_4=\\lambda_5=0$, so $-\\lambda_3=2x_3=2\\implies\\lambda_3=-2<0$, so the KKT conditions fail.\n",
    "\n",
    " * Case 1-3:\n",
    " $x_2=1$, $x_3=0$, then $\\lambda_3=\\lambda_6=0$, so $\\lambda_4=-6\\implies\\lambda_4<0$, so the KKT conditions fail.\n",
    "\n",
    " * Case 1-4:\n",
    " $x_2=1$, $x_3=1$, then $\\lambda_3=\\lambda_5=0$, so $\\lambda_6=2-6=-4\\implies\\lambda_6<0$, so the KKT conditions fail.  \n",
    "\n",
    "  \n",
    "* Case 2:\n",
    "$x_1 = 1$, then $\\lambda_1=0$,\n",
    "\n",
    " * Case 2-1:\n",
    " $x_2=0$, $x_3=0$, then $\\lambda_4=\\lambda_6=0$, so $-\\lambda_3=2-0+0=2\\implies\\lambda_3<0$, so the KKT conditions fail.\n",
    "\n",
    " * Case 2-2:\n",
    " $x_2=0$, $x_3=1$, then $\\lambda_4=\\lambda_5=0$, so $-\\lambda_3=2-0+2=4\\implies\\lambda_3<0$, so the KKT conditions fail.\n",
    "\n",
    " * Case 2-3:\n",
    " $x_2=1$, $x_3=0$, then $\\lambda_3=\\lambda_6=0$, so $-\\lambda_5=2-0=2\\implies\\lambda_5<0$, so the KKT conditions fail.\n",
    "\n",
    " * Case 2-4:\n",
    " $x_2=1$, $x_3=1$, then $\\lambda_4=\\lambda_5=0$, so $\\lambda_6=2-6=-4\\implies\\lambda_6<0$, so the KKT conditions fail.  \n",
    "\n",
    "  \n",
    "* Case 3:\n",
    "$\\lambda_1=\\lambda_2=0$ and $x_1\\neq 0$ or $1$, then $6x_1=2x_2\\implies3x_1=x_2$, then we will have $x_2\\neq0\\implies\\lambda_3=0$.\n",
    "\n",
    " * Case 3-1:\n",
    " if $x_2=1$ and $x_1=\\frac{1}{3}$, then $\\frac{2}{3}-6+2x_3=\\lambda_4$. Since $x_3\\leq1$, then $2x_3\\leq2$, implies that $\\frac{2}{3}-6+2x_3=\\lambda_4<0$, so the KKT conditions fail.   \n",
    " \n",
    " * Case 3-2:\n",
    " if $x_2<1$, then $\\lambda_3=\\lambda_4=0$, so $2x_1-6x_2+2x_3=0=-16x_1+2x_3$. And also $\\lambda_5,\\lambda_6$ cannot be $0$ at the same time in this case, so $x_3=0$ or $1$. $x_3$ cannot be $0$ since $x_1\\neq 0$ and $0=-16x_1+2x_3$. Then $x_3=1$, so $x_1=\\frac{1}{8}$, and $x_2=\\frac{3}{8}$, and $\\lambda_1=\\lambda_2=\\lambda_3=\\lambda_4=\\lambda_5=0$, $\\lambda_6=2x_2-6x_3=\\frac{3}{4}-6<0$, so the KKT conditions fail.  \n",
    " \n",
    "\n",
    "* Case 4:\n",
    "$\\lambda_1=\\lambda_2=0$ and $x_1= 0$ or $1$, then $6x_1=2x_2\\implies3x_1=x_2$, since $x_2\\leq 1$, $x_1\\neq 1$, so $x_1=x_2=0\\implies\\lambda_4=0$. In order to avoid duplication of cases, $x_3\\neq 0$.  \n",
    "Then $2x_3=-\\lambda_3$. Since $0< x_3\\leq 1$, then $\\lambda_3<0$, so the KKT conditions fail.   \n",
    "\n",
    "\n",
    "* Case 5:\n",
    "$\\lambda_3=\\lambda_4=0$ and $x_2\\neq 0$ or $1$, then $2x_1-6x_2+2x_3=0\\implies2x_3=6x_2-2x_1$. In order to avoid duplication of cases, $\\lambda_1, \\lambda_2\\neq 0$ at the same time.\n",
    "\n",
    " * Case 5-1:\n",
    " $x_1=0, \\lambda_2=0$, then $2x_2=-\\lambda_1\\implies\\lambda_1<0$, so the KKT conditions fail.   \n",
    " \n",
    " * Case 5-2:\n",
    " $x_1=1, \\lambda_1=0$, then $2x_2-6=\\lambda_2\\implies\\lambda_2<0$, so the KKT conditions fail.   \n",
    " \n",
    " \n",
    "* Case 6:\n",
    "$\\lambda_3=\\lambda_4=0$ and $x_2=0$ or $1$, then $2x_1-6x_2+2x_3=0\\implies2x_3=6x_2-2x_1$. In order to avoid duplication of cases, $\\lambda_1, \\lambda_2\\neq 0$ at the same time.\n",
    "\n",
    " * Case 6-1:\n",
    " $x_2=0$, then $2x_3=-2x_1$, and we have $x_1=0$ or $1$. if $x_1=0$, then $x_2=0$, $x_3=0$, this is the same as Case 1-1. If $x_1=1$, $x_3<0$, so the KKT conditions fail.  \n",
    " \n",
    " * Case 6-2:\n",
    " $x_2=1$, then $2x_3=6-2x_1$. Since $x_1=0$ or $1$, then $2x_3=6$ or $4$. In both cases, $x_3$ is not in the feasible range, so the KKT conditions fail.  \n",
    " \n",
    "\n",
    "* Case 7:\n",
    "$\\lambda_5=\\lambda_6=0$ and $x_3\\neq 0$ or $1$, then $6x_3=2x_2\\implies3x_3=x_2$, then we will have $x_2\\neq0\\implies\\lambda_3=0$.\n",
    "\n",
    " * Case 7-1:\n",
    " if $x_2=1$ and $x_3=\\frac{1}{3}$, then $\\frac{2}{3}-6+2x_1=\\lambda_4$. Since $x_1\\leq1$, then $2x_1\\leq2$, implies that $\\frac{2}{3}-6+2x_1=\\lambda_4<0$, so the KKT conditions fail.   \n",
    " \n",
    " * Case 7-2:\n",
    " if $x_2<1$, then $\\lambda_3=\\lambda_4=0$, so $2x_1-6x_2+2x_3=0=-16x_3+2x_1$. And also $\\lambda_1,\\lambda_2$ cannot be $0$ at the same time in this case, so $x_1=0$ or $1$. $x_1$ cannot be $0$ since $x_3\\neq 0$ and $0=-16x_1+2x_3$. Then $x_1=1$, so $x_3=\\frac{1}{8}$, and $x_2=\\frac{3}{8}$, and $\\lambda_2=\\lambda_3=\\lambda_4=\\lambda_5=\\lambda_6=0$, $-\\lambda_1=2x_2-6x_1=\\frac{3}{4}-6<0$, so the KKT conditions fail.  \n",
    " \n",
    "\n",
    "* Case 8:\n",
    "$\\lambda_5=\\lambda_6=0$ and $x_3= 0$ or $1$, then $6x_3=2x_2\\implies3x_3=x_2$, since $x_2\\leq 1$, $x_3\\neq 1$, so $x_3=x_2=0\\implies\\lambda_4=0$. In order to avoid duplication of cases, $x_1\\neq 0$.  \n",
    "Then $2x_1=-\\lambda_3$. Since $0< x_1\\leq 1$, then $\\lambda_3<0$, so the KKT conditions fail.   \n",
    "  \n",
    "\n",
    "Therefore, we can get that as $x_1=0,x_2=0,x_3=0$, $x=\\begin{pmatrix} 0 \\\\ 0 \\\\ 0\\end{pmatrix}$ is the only point that satisfies the KKT conditions."
   ]
  },
  {
   "cell_type": "markdown",
   "metadata": {
    "collapsed": true
   },
   "source": [
    "### Part (d)\n",
    "\n",
    "** $x=\\begin{pmatrix} 0 \\\\ 0 \\\\ 0\\end{pmatrix}$ is the solution to this program** not only because that $x=\\begin{pmatrix} 0 \\\\ 0 \\\\ 0\\end{pmatrix}$ is the only point that satisfies the KKT conditions, but also:  \n",
    "\n",
    "Consider the program  \n",
    "$$\n",
    "\\min_{x\\in\\mathbb{R^2}}3x_1^2-2x_1x_2+3x_2^2-2x_2x_3+3x_3^2 \\text{ subject to } 0\\leq x_1\\leq1, 0\\leq x_2\\leq1, 0\\leq x_3\\leq1\n",
    "$$  \n",
    "then, observe that  \n",
    "$$\n",
    "f(x_1,x_2,x_3)=3x_1^2-2x_1x_2+3x_2^2-2x_2x_3+3x_3^2 = (x_1-x_2)^2+(x_2-x_3)^2+2x_1^2+x_2^2+2x_3^2\n",
    "$$  \n",
    "We know that $(x_1-x_2)^2\\geq 0$, $(x_2-x_3)^2\\geq 0$, $2x_1^2\\geq 0$, $x_2^2\\geq 0$, $2x_3^2\\geq 0$, so  \n",
    "$$\n",
    "(x_1-x_2)^2+(x_2-x_3)^2+2x_1^2+x_2^2+2x_3^2 \\geq 0\n",
    "$$  \n",
    "So the minimum value of $f(x_1,x_2,x_3)$ is $0$. Then the minimum value occurs as $(x_1-x_2)^2=0$, $(x_2-x_3)^2=0$, $2x_1^2=0$, $x_2^2=0$, $2x_3^2=0$, which means  \n",
    "$$\n",
    "x_1=0, x_2=0, x_3=0. \n",
    "$$  \n",
    "Thus, $x=\\begin{pmatrix} 0 \\\\ 0 \\\\ 0\\end{pmatrix}$ is the solution to this program."
   ]
  },
  {
   "cell_type": "markdown",
   "metadata": {},
   "source": [
    "**********************************"
   ]
  }
 ],
 "metadata": {
  "kernelspec": {
   "display_name": "Python 3",
   "language": "python",
   "name": "python3"
  },
  "language_info": {
   "codemirror_mode": {
    "name": "ipython",
    "version": 3
   },
   "file_extension": ".py",
   "mimetype": "text/x-python",
   "name": "python",
   "nbconvert_exporter": "python",
   "pygments_lexer": "ipython3",
   "version": "3.6.1"
  }
 },
 "nbformat": 4,
 "nbformat_minor": 2
}
